implicit arguments for equal (to do:  existH, etc.)

theories/ordinals/Ackermann/LNT.v
@@ -15,7 +15,6 @@ Definition Sentence := Sentence LNT.
 Definition Term := Term LNT.
 Definition Terms := Terms LNT.
 Definition var := var LNT.
-Definition equal := equal LNT.
 Definition existH := existH LNT.
 Definition ifThenElseH := ifThenElseH LNT.
 Definition SysPrf := SysPrf LNT.
