theories/ordinals/Ackermann/NN2PA.v
@@ -79,7 +79,7 @@ simple induction m.
                (LNN2LNT_formula
                   (impH (LNN.LT (fol.var LNN x) (LNN.Succ (LNN.natToTerm n)))
                      (orH (LNN.LT (fol.var LNN x) (LNN.natToTerm n))
-                        (LNN.equal (fol.var LNN x) (LNN.natToTerm n))))))
+                        (equal (fol.var LNN x) (LNN.natToTerm n))))))
       by (apply NN2PA, nn8). 
       simpl in H1; simpl. 
       unfold orH, fol.orH; apply H1.
