theories/ordinals/Ackermann/fol.v
@@ -718,7 +718,7 @@ Arguments notH {L} _.
 Arguments forallH {L} _ _.
 Arguments orH {L} _ _.
 Arguments andH {L} _ _.
-(* To compile *)
 Arguments iffH {L} _ _.
+Arguments equal {L} _ _.
 
 
